$$k_1 = \alpha + \beta_i$$
$$k_2 = \alpha - \beta_i$$

Пример:
$$y''' + 3y'' + 9y' - 13y = 0$$
$$k^3 + 3k^2 + 9k - 13 = 0$$
Подбором нашли k = 1 - корень.

|       | 1   | 3   | 9   | -13 |
| ----- | --- | --- | --- | --- |
| k = 1 | 1   | 4   | 13  | 0   |

$$(k-1)(k^2 + 4k + 13) = 0$$
$$(k^2 + 4k + 13) = 0$$
$$D = 16 - 52 = -36$$
$$k_{1,2} = \frac{-4 \pm \sqrt{-36}}{-2 +-3i}$$
$$k_{1,2} = -2 \pm3i$$
$$y_1 =e^x$$
$$y_2 =e^{-2x}cos3x$$
$$y_3 =e^{-2x}sin3x$$

### 721

$$
y'' - 6y' + 8y = 0\\
k^2 - 6k + 8 = 0\\
k = 2; k = 4 \\
y_1 = e^2x
$$

$$y_1 = e^4x $$

### 777

| $e^x$ | $e^{-2x}cos3x$                                                   | $e^{-2x}sin3x$                                                 |
| ----- | ---------------------------------------------------------------- | -------------------------------------------------------------- |
| $e^x$ | $-2e^{-2x}cos3x - e^{-2x}3sin(3x)$                               | $-2e^{-2x} sin(3x) + 3e^{-2x}cos(3x)$                          |
| $e^x$ | $4e^{-2x}cos3x -2e^{-2x}(-3)sin(3x)+6e^{-2x}sin3x-9e^{-2x}cos3x$ | $4e^{-2x}sin3x - 6e^{-2x}cos3x -6e^{-2x}cos3x - 9e^{-2x}sin3x$ |

Находим определитель и получаем $54e^{-3x}=>$,следовательно образует систему фундаментальных решений
