\documentclass{article}
\usepackage{amsmath}
\usepackage{tikz}

\begin{document}

\section*{Page 1}

\[
x + 2y/3 - z/3 = 0
\]

1. 

\[
3x - 2y - z = 0 \quad \text{(1)}
\]

2. 
\[
M_1 \text{: Substituting values to satisfy (1)}
\]

\[
\text{2: Substitute and solve}
\]

3. 

\[
3x - 2y = 0 \quad \text{and} \quad 2x + 3y + z/3 = 0
\]

\[
\left\{
\begin{array}{l}
2x + 3y = -3 \\
3y - 2z = -2
\end{array}
\right\}
\]

Solving the system:
\[
\left\{
\begin{array}{ccc}
2 & 3 & -3 \\
3 & -2 & -2 
\end{array}
\right\}
\]

\[
\text{Result: } x = 0, \quad y = -1
\]

4. 

\[
3x - 2y - z = 0 \quad \text{and} \quad 8x + 12 = x + z/3
\]

\[
x = \frac{2}{3}(y + 1)
\]

\[
64 + 144y = x + y + z/3
\]

\[
x = \frac{2}{3}(y+1), \quad y = 0, \quad z = 2
\]

\[
M: (0, -1, 0)
\]

5. 

\[
x = \frac{2}{3}(y+1)
\]

\[
y = \frac{3}{4}(y + 1)^2
\]

\[
64 = x + y + z/3
\]

\section*{Page 2}

Given: 

\[
A(1, -2), \quad B(4, -4), \quad C(1, -2)
\]

1. 

\[
\text{Find the midpoint } M \text{ of } AB
\]

\begin{tikzpicture}
\draw (0,0) -- (2,3) -- (4,0) -- cycle;
\draw[dashed] (2,3) -- (2,0);
\node at (2,3.2) {A};
\node at (4.2,0) {B};
\node at (-0.2,0) {C};
\node at (2,-0.2) {M};
\end{tikzpicture}

\[
AM : \frac{x-3}{2} = \frac{y-1}{-1}
\]

Answer:

Given: 

\[
M(2,1,1)
\]

\[
E: 2x + 3y + 3z = 6
\]

\[
\text{Vector Normal} \left\{
\begin{array}{l}
x = 2 \\
y = 3 \\
z = 6
\end{array}
\right\}
\]

Solution:

1. 

\[
\text{Vector Normal of E is perpendicular to M}
\]

\end{document}
